theories/swap_later_impl.v
@@ -143,13 +143,13 @@ Proof.
 Qed.
 
 (** ** Dependently-typed functions over a finite discrete domain *)
-Instance Swappable_ofe_funUR {A} (B: A → ucmraT) (H: ∀ i, CmraSwappable (B i)): CmraSwappable (ofe_funUR B).
+Instance Swappable_ofe_funUR {A} (B: A → ucmraT) (H: ∀ i, CmraSwappable (B i)): CmraSwappable (discrete_funUR B).
 Proof.
   split => n mx z Hvmx Hvzmx.
   unshelve eassert (FUN := λ a, cmra_extend_included n (($ a) <$> mx) (z a) _ _).
-  1-2: move: Hvzmx; destruct mx; rewrite /= -?ofe_fun_lookup_op ?Some_validN; eauto.
+  1-2: move: Hvzmx; destruct mx; rewrite /= -?discrete_fun_lookup_op ?Some_validN; eauto.
   exists (λ x, proj1_sig (FUN x)); split_and! => a;
-  destruct mx; rewrite /= ?ofe_fun_lookup_op //; destruct (FUN a) as (?&HP1&HP2); eauto.
+  destruct mx; rewrite /= ?discrete_fun_lookup_op //; destruct (FUN a) as (?&HP1&HP2); eauto.
 
   (* Alternative proof. *)
   (* Restart.
@@ -157,7 +157,7 @@ Proof.
   split => n [x|] /= z Hvmx Hvzmx.
   - assert (FUN := λ a, cmra_extend_included n (Some (x a)) (z a) (Hvmx a) (Hvzmx a)).
     exists (λ x, proj1_sig (FUN x)); split_and! => a;
-    rewrite /= ?ofe_fun_lookup_op //; by destruct (FUN a) as (?&?&?).
+    rewrite /= ?discrete_fun_lookup_op //; by destruct (FUN a) as (?&?&?).
   - assert (FUN := λ a, cmra_extend_included n None (z a) I (Hvzmx a)).
     exists (λ x, proj1_sig (FUN x)); split_and! => a;
     by destruct (FUN a) as (?&?&?). *)
